theories/Rename.v
@@ -12,22 +12,22 @@ From LinearCore Require Import
 
 
 
-Inductive Strict (lookup : Map.to Name.name) : Pattern.strict -> Pattern.strict -> Prop :=
+Inductive Strict {lookup : Map.to Name.name} (O2O : Map.OneToOne lookup) : Pattern.strict -> Pattern.strict -> Prop :=
   | SCtr ctor
-      : Strict lookup (Pattern.Ctr ctor) (Pattern.Ctr ctor)
+      : Strict O2O (Pattern.Ctr ctor) (Pattern.Ctr ctor)
   | SApp
       argument renamed_argument unused (rename_argument : Map.Pop lookup argument renamed_argument unused)
-      curried renamed_curried (rename_curried : Strict unused curried renamed_curried)
-      : Strict lookup (Pattern.App curried argument) (Pattern.App renamed_curried renamed_argument)
+      (O2OU : Map.OneToOne unused) curried renamed_curried (rename_curried : Strict O2OU curried renamed_curried)
+      : Strict O2O (Pattern.App curried argument) (Pattern.App renamed_curried renamed_argument)
   .
-Arguments Strict lookup strict renamed_strict.
+Arguments Strict {lookup} O2O strict renamed_strict.
 
 Lemma strict_eq
-  {l1 s1 r1} (S1 : Strict l1 s1 r1)
-  {l2} (El : Map.Eq l1 l2)
+  {l1} {O2O1 : Map.OneToOne l1} {s1 r1} (S1 : Strict O2O1 s1 r1)
+  {l2} (El : Map.Eq l1 l2) (O2O2 : Map.OneToOne l2)
   {s2} (Es : s1 = s2)
   {r2} (Er : r1 = r2)
-  : Strict l2 s2 r2.
+  : Strict O2O2 s2 r2.
 Proof.
   subst. generalize dependent l2. induction S1; intros. { constructor. }
   econstructor. { eapply Map.pop_eq; try reflexivity; try eassumption. apply Map.eq_refl. } exact S1.
@@ -44,22 +44,23 @@ Fixpoint strict lookup s :=
       end
   end.
 
-Lemma strict_spec lookup s
-  : Reflect.Option (Strict lookup s) (strict lookup s).
+Lemma strict_spec {lookup} (O2O : Map.OneToOne lookup) s
+  : Reflect.Option (Strict O2O s) (strict lookup s).
 Proof.
   generalize dependent lookup. induction s; intros; cbn in *. { constructor. constructor. }
   fold (Map.pop lookup argument). destruct (Map.pop_spec lookup argument) as [[renamed_argument unused] |]. 2: {
-    constructor. intros p S. invert S. apply (N (_, _)) in rename_argument as []. }
-  specialize (IHs unused). destruct IHs; constructor. { econstructor. { exact Y. } exact Y0. }
+    constructor. intros p S. invert S. apply (N (_, _)) in rename_argument as []. } simpl fst in *. simpl snd in *.
+  assert (O2OU : Map.OneToOne unused). { eapply Map.one_to_one_remove_if_present. { exact O2O. } apply Y. }
+  specialize (IHs _ O2OU). destruct IHs; constructor. { econstructor. { exact Y. } exact Y0. }
   intros p C. invert C. eapply N. eapply strict_eq; try reflexivity. { exact rename_curried. }
   eapply Map.pop_det; try reflexivity; try eassumption. apply Map.eq_refl.
 Qed.
 
 Lemma strict_det
-  {l1 s1 r1} (S1 : Strict l1 s1 r1)
-  {l2} (El : Map.Eq l1 l2)
+  {l1} {O2O1 : Map.OneToOne l1} {s1 r1} (S1 : Strict O2O1 s1 r1)
+  {l2} (El : Map.Eq l1 l2) (O2O2 : Map.OneToOne l2)
   {s2} (Es : s1 = s2)
-  {r2} (S2 : Strict l2 s2 r2)
+  {r2} (S2 : Strict O2O2 s2 r2)
   : r1 = r2.
 Proof.
   subst. generalize dependent r2. generalize dependent l2.
@@ -69,13 +70,15 @@ Proof.
 Qed.
 
 Definition CompatibleStrict (lookup : Map.to Name.name) strict : Prop :=
+  Map.OneToOne lookup /\
   WellFormed.Strict strict /\
   Map.Subset (BoundIn.strict strict) (Map.domain lookup).
 
-Lemma compatible_if_strict {lookup strict renamed_strict} (S : Strict lookup strict renamed_strict)
+Lemma compatible_if_strict {lookup} {O2O : Map.OneToOne lookup} {strict renamed_strict} (S : Strict O2O strict renamed_strict)
   : CompatibleStrict lookup strict.
 Proof.
-  induction S. { split. { constructor. } intros k v F. invert F. } destruct IHS as [WF SS]. constructor.
+  induction S. { split. { exact O2O. } split. { constructor. } intros k v F. invert F. }
+  destruct IHS as [O2OU' [WF SS]]. split. { exact O2O. } split.
   - constructor. { exact WF. } intro B. apply BoundIn.strict_spec in B as [[] B]. apply SS in B.
     apply Map.find_domain in B as [name B]. apply rename_argument in B as [N _]. apply N. reflexivity.
   - intros k v F. apply Map.find_domain. cbn in F. apply Map.find_overriding_add in F as [[-> ->] | [N F]].
@@ -85,31 +88,56 @@ Qed.
 
 Lemma strict_iff_compatible lookup strict
   : CompatibleStrict lookup strict <->
-    exists renamed_strict, Strict lookup strict renamed_strict.
+    exists (O2O : Map.OneToOne lookup) renamed_strict,
+    Strict O2O strict renamed_strict.
 Proof.
   generalize dependent lookup. induction strict; intros.
-  - split. { intros [WF S]. eexists. constructor. }
-    intros [renamed_strict S]. split. { constructor. } intros k v F. invert F.
-  - split. 2: { intros [renamed_strict S]. eapply compatible_if_strict. exact S. }
-    intros [WF S]. invert WF. assert (A := S). eapply Map.find_domain in A as [renamed_argument A]. 2: {
+  - split. { intros [O2O [WF S]]. exists O2O. eexists. constructor. }
+    intros [O2O [renamed_strict S]]. split. { exact O2O. } split. { constructor. } intros k v F. invert F.
+  - split. 2: { intros [O2O [renamed_strict S]]. eapply compatible_if_strict. exact S. }
+    intros [O2O [WF S]]. invert WF. assert (A := S). eapply Map.find_domain in A as [renamed_argument A]. 2: {
       apply Map.find_overriding_add. left. split; reflexivity. }
-    assert (C : CompatibleStrict (Map.remove argument lookup) strict0). { split. { exact curried_well_formed. }
-      intros k v F. apply Map.find_domain. eapply Map.in_remove_if_present. { apply Map.remove_if_present_remove. }
+    assert (C : CompatibleStrict (Map.remove argument lookup) strict0). {
+      split. { eapply Map.one_to_one_remove_if_present. 2: { apply Map.remove_if_present_remove. } exact O2O. }
+      split. { exact curried_well_formed. } intros k v F. apply Map.find_domain.
+      eapply Map.in_remove_if_present. { apply Map.remove_if_present_remove. }
       assert (Nk : k <> argument). { intros ->. apply N. apply BoundIn.strict_spec. eexists. exact F. }
       split. { exact Nk. } eapply Map.find_domain. apply S. cbn. apply Map.find_overriding_add.
       right. split. { exact Nk. } exact F. }
-    apply IHstrict in C as [renamed_strict C]. eexists. econstructor. 2: { exact C. }
+    apply IHstrict in C as [O2OR [renamed_strict C]]. exists O2O. eexists. econstructor. 2: { exact C. }
     split. { exact A. } apply Map.remove_if_present_remove.
+Qed.
+
+Lemma strict_reversible {lookup} (O2O : Map.OneToOne lookup) {inverted} (inv : Map.Invert lookup inverted)
+  (O2OI : Map.OneToOne inverted) strict renamed_strict
+  : Strict O2O strict renamed_strict <-> Strict O2OI renamed_strict strict.
+Proof. { split; intro S.
+  - generalize dependent inverted. induction S; intros; econstructor.
+    + destruct rename_argument as [F R]. split. { apply inv. exact F. } apply Map.remove_if_present_remove.
+    + apply IHS. intros k v. assert (A := @Map.remove_if_present_remove); cbn in A; rewrite A; clear A.
+      destruct rename_argument as [F R]. cbn in R. rewrite R. split; (intros [N F']; split; [| apply inv; exact F']).
+      * intros ->. apply N. eapply O2O; eassumption.
+      * intros ->. apply N. apply inv in F'. eapply Map.find_det; eassumption.
+  - generalize dependent lookup. induction S; intros; econstructor.
+    + destruct rename_argument as [F R]. split. { apply inv. exact F. } apply Map.remove_if_present_remove.
+    + apply IHS. intros k v. assert (A := @Map.remove_if_present_remove); cbn in A; rewrite A; clear A.
+      destruct rename_argument as [F R]. cbn in R. rewrite R. split; (intros [N F']; split; [| apply inv; exact F']).
+      * intros ->. apply N. apply inv in F'. eapply Map.find_det; eassumption.
+      * intros ->. apply N. eapply O2O; eassumption. }
+  Unshelve.
+  - eapply Map.one_to_one_remove_if_present. 2: { apply Map.remove_if_present_remove. } exact O2OI.
+  - eapply Map.one_to_one_remove_if_present. 2: { apply Map.remove_if_present_remove. } exact O2O0.
 Qed.
 
 
 
-Variant MoveOrReference lookup : Pattern.move_or_reference -> Pattern.move_or_reference -> Prop :=
-  | MMov strict renamed_strict (rename_strict : Strict lookup strict renamed_strict)
-      : MoveOrReference lookup (Pattern.Mov strict) (Pattern.Mov renamed_strict)
-  | MRef strict renamed_strict (rename_strict : Strict lookup strict renamed_strict)
-      : MoveOrReference lookup (Pattern.Ref strict) (Pattern.Ref renamed_strict)
+Variant MoveOrReference {lookup} (O2O : Map.OneToOne lookup) : Pattern.move_or_reference -> Pattern.move_or_reference -> Prop :=
+  | MMov strict renamed_strict (rename_strict : Strict O2O strict renamed_strict)
+      : MoveOrReference O2O (Pattern.Mov strict) (Pattern.Mov renamed_strict)
+  | MRef strict renamed_strict (rename_strict : Strict O2O strict renamed_strict)
+      : MoveOrReference O2O (Pattern.Ref strict) (Pattern.Ref renamed_strict)
   .
+Arguments MoveOrReference {lookup} O2O pattern renamed_pattern.
 
 Definition move_or_reference lookup mr :=
   match mr with
@@ -117,27 +145,27 @@ Definition move_or_reference lookup mr :=
   | Pattern.Ref s => option_map Pattern.Ref (strict lookup s)
   end.
 
-Lemma move_or_reference_spec lookup mr
-  : Reflect.Option (MoveOrReference lookup mr) (move_or_reference lookup mr).
+Lemma move_or_reference_spec {lookup} (O2O : Map.OneToOne lookup) mr
+  : Reflect.Option (MoveOrReference O2O mr) (move_or_reference lookup mr).
 Proof.
-  destruct mr; cbn; (destruct (strict_spec lookup strict0); constructor; [constructor; exact Y |]);
+  destruct mr; cbn; (destruct (strict_spec O2O strict0); constructor; [constructor; exact Y |]);
   intros s M; invert M; apply N in rename_strict as [].
 Qed.
 
 Lemma move_or_reference_det
-  {l1 mr1 r1} (MR1 : MoveOrReference l1 mr1 r1)
-  {l2} (El : Map.Eq l1 l2)
+  {l1} {O2O1 : Map.OneToOne l1} {mr1 r1} (MR1 : MoveOrReference O2O1 mr1 r1)
+  {l2} (El : Map.Eq l1 l2) (O2O2 : Map.OneToOne l2)
   {mr2} (Emr : mr1 = mr2)
-  {r2} (MR2 : MoveOrReference l2 mr2 r2)
+  {r2} (MR2 : MoveOrReference O2O2 mr2 r2)
   : r1 = r2.
 Proof. invert MR1; invert MR2; f_equal; eapply strict_det; try reflexivity; eassumption. Qed.
 
 Lemma move_or_reference_eq
-  {l1 mr1 r1} (MR1 : MoveOrReference l1 mr1 r1)
-  {l2} (El : Map.Eq l1 l2)
+  {l1} {O2O1 : Map.OneToOne l1} {mr1 r1} (MR1 : MoveOrReference O2O1 mr1 r1)
+  {l2} (El : Map.Eq l1 l2) (O2O2 : Map.OneToOne l2)
   {mr2} (Emr : mr1 = mr2)
   {r2} (Er : r1 = r2)
-  : MoveOrReference l2 mr2 r2.
+  : MoveOrReference O2O2 mr2 r2.
 Proof. subst. invert MR1; constructor; eapply strict_eq; try reflexivity; eassumption. Qed.
 
 Variant CompatibleMoveOrReference lookup : Pattern.move_or_reference -> Prop :=
@@ -149,24 +177,30 @@ Variant CompatibleMoveOrReference lookup : Pattern.move_or_reference -> Prop :=
 
 Lemma move_or_reference_iff_compatible lookup move_or_reference
   : CompatibleMoveOrReference lookup move_or_reference <->
-    exists renamed_move_or_reference, MoveOrReference lookup move_or_reference renamed_move_or_reference.
+    exists (O2O : Map.OneToOne lookup) renamed_move_or_reference,
+    MoveOrReference O2O move_or_reference renamed_move_or_reference.
 Proof.
   split.
-  - intro C. invert C; apply strict_iff_compatible in CS as [renamed_strict S]; eexists; constructor; exact S.
-  - intros [renamed_move_or_reference MR].
-    invert MR; constructor; apply strict_iff_compatible; eexists; exact rename_strict.
+  - intro C. invert C; apply strict_iff_compatible in CS as [O2O [renamed_strict S]]; exists O2O; eexists; constructor; exact S.
+  - intros [O2O [renamed_move_or_reference MR]].
+    invert MR; constructor; apply strict_iff_compatible; exists O2O; eexists; exact rename_strict.
 Qed.
 
+Lemma move_or_reference_reversible {lookup} (O2O : Map.OneToOne lookup) {inverted} (inv : Map.Invert lookup inverted)
+  (O2OI : Map.OneToOne inverted) move_or_reference renamed_move_or_reference
+  : MoveOrReference O2O move_or_reference renamed_move_or_reference <-> MoveOrReference O2OI renamed_move_or_reference move_or_reference.
+Proof. split; intro MR; invert MR; constructor; eapply strict_reversible; try eassumption; apply Map.invert_sym; assumption. Qed.
 
 
-Variant Pattern lookup : Pattern.pattern -> Pattern.pattern -> Prop :=
+
+Variant Pattern {lookup} (O2O : Map.OneToOne lookup) : Pattern.pattern -> Pattern.pattern -> Prop :=
   | Nam name renamed (rename_name : Map.Find lookup name renamed)
-      : Pattern lookup (Pattern.Nam name) (Pattern.Nam renamed)
+      : Pattern O2O (Pattern.Nam name) (Pattern.Nam renamed)
   | Pat move_or_reference renamed_move_or_reference
-      (rename_move_or_reference : MoveOrReference lookup move_or_reference renamed_move_or_reference)
-      : Pattern lookup (Pattern.Pat move_or_reference) (Pattern.Pat renamed_move_or_reference)
+      (rename_move_or_reference : MoveOrReference O2O move_or_reference renamed_move_or_reference)
+      : Pattern O2O (Pattern.Pat move_or_reference) (Pattern.Pat renamed_move_or_reference)
   .
-Arguments Pattern lookup pattern renamed_pattern.
+Arguments Pattern {lookup} O2O pattern renamed_pattern.
 
 Definition pattern lookup patt :=
   match patt with
@@ -174,21 +208,21 @@ Definition pattern lookup patt :=
   | Pattern.Pat mr => option_map Pattern.Pat (move_or_reference lookup mr)
   end.
 
-Lemma pattern_spec lookup patt
-  : Reflect.Option (Pattern lookup patt) (pattern lookup patt).
+Lemma pattern_spec {lookup} (O2O : Map.OneToOne lookup) patt
+  : Reflect.Option (Pattern O2O patt) (pattern lookup patt).
 Proof.
   destruct patt; cbn in *.
   - destruct (Map.find_spec lookup name); constructor. { constructor. exact Y. }
     intros p P. invert P. apply N in rename_name as [].
-  - destruct (move_or_reference_spec lookup move_or_reference0); constructor. { constructor. exact Y. }
+  - destruct (move_or_reference_spec O2O move_or_reference0); constructor. { constructor. exact Y. }
     intros p P. invert P. apply N in rename_move_or_reference as [].
 Qed.
 
 Lemma pattern_det
-  {l1 p1 r1} (P1 : Pattern l1 p1 r1)
-  {l2} (El : Map.Eq l1 l2)
+  {l1} {O2O1 : Map.OneToOne l1} {p1 r1} (P1 : Pattern O2O1 p1 r1)
+  {l2} (El : Map.Eq l1 l2) (O2O2 : Map.OneToOne l2)
   {p2} (Ep : p1 = p2)
-  {r2} (P2 : Pattern l2 p2 r2)
+  {r2} (P2 : Pattern O2O2 p2 r2)
   : r1 = r2.
 Proof.
   invert P1; invert P2; f_equal. { eapply Map.find_det. { eassumption. } apply El. assumption. }
@@ -196,27 +230,27 @@ Proof.
 Qed.
 
 Lemma pattern_eq
-  {l1 p1 r1} (P1 : Pattern l1 p1 r1)
-  {l2} (El : Map.Eq l1 l2)
+  {l1} {O2O1 : Map.OneToOne l1} {p1 r1} (P1 : Pattern O2O1 p1 r1)
+  {l2} (El : Map.Eq l1 l2) (O2O2 : Map.OneToOne l2)
   {p2} (Ep : p1 = p2)
   {r2} (Er : r1 = r2)
-  : Pattern l2 p2 r2.
+  : Pattern O2O2 p2 r2.
 Proof.
   subst. invert P1; constructor. { apply El. exact rename_name. }
   eapply move_or_reference_eq; try reflexivity; eassumption.
 Qed.
 
-Lemma pattern_iff lookup patt renamed_patt
-  : Pattern lookup patt renamed_patt <-> pattern lookup patt = Some renamed_patt.
+Lemma pattern_iff {lookup} (O2O : Map.OneToOne lookup) patt renamed_patt
+  : Pattern O2O patt renamed_patt <-> pattern lookup patt = Some renamed_patt.
 Proof.
-  destruct (pattern_spec lookup patt).
+  destruct (pattern_spec O2O patt).
   - split. 2: { intro E. invert E. exact Y. }
     intro P. f_equal. eapply pattern_det; try reflexivity; try eassumption. apply Map.eq_refl.
   - split. { intro P. apply N in P as []. } intro D. discriminate D.
 Qed.
 
 Variant CompatiblePattern lookup : Pattern.pattern -> Prop :=
-  | CNam name (I : Map.In lookup name)
+  | CNam (O2O : Map.OneToOne lookup) name (I : Map.In lookup name)
       : CompatiblePattern lookup (Pattern.Nam name)
   | CPat move_or_reference (C : CompatibleMoveOrReference lookup move_or_reference)
       : CompatiblePattern lookup (Pattern.Pat move_or_reference)
@@ -224,122 +258,316 @@ Variant CompatiblePattern lookup : Pattern.pattern -> Prop :=
 
 Lemma pattern_iff_compatible lookup pattern
   : CompatiblePattern lookup pattern <->
-    exists renamed_pattern, Pattern lookup pattern renamed_pattern.
+    exists (O2O : Map.OneToOne lookup) renamed_pattern, Pattern O2O pattern renamed_pattern.
 Proof.
   split.
   - intro CP. invert CP.
-    + destruct I as [y F]. eexists. constructor. exact F.
-    + apply move_or_reference_iff_compatible in C as [renamed_move_or_reference C].
-      eexists. constructor. exact C.
-  - intros [renamed_pattern P]. invert P. { constructor. eexists. exact rename_name. }
-    constructor. apply move_or_reference_iff_compatible. eexists. exact rename_move_or_reference.
+    + exists O2O. destruct I as [y F]. eexists. constructor. exact F.
+    + apply move_or_reference_iff_compatible in C as [O2O [renamed_move_or_reference C]].
+      exists O2O. eexists. constructor. exact C.
+  - intros [O2O [renamed_pattern P]]. invert P. { constructor. { exact O2O. } eexists. exact rename_name. }
+    constructor. apply move_or_reference_iff_compatible. exists O2O. eexists. exact rename_move_or_reference.
+Qed.
+
+Lemma pattern_reversible {lookup} (O2O : Map.OneToOne lookup) {inverted} (inv : Map.Invert lookup inverted)
+  (O2OI : Map.OneToOne inverted) pattern renamed_pattern
+  : Pattern O2O pattern renamed_pattern <-> Pattern O2OI renamed_pattern pattern.
+Proof.
+  split; intro P.
+  - generalize dependent inverted. induction P; intros. { constructor. apply inv. exact rename_name. }
+    constructor. eapply move_or_reference_reversible. { apply Map.invert_sym. eassumption. } eassumption.
+  - generalize dependent lookup. induction P; intros. { constructor. apply inv. exact rename_name. }
+    constructor. eapply move_or_reference_reversible; eassumption.
 Qed.
 
 
 
-Inductive Term (lookup : Map.to Name.name) : Term.term -> Term.term -> Prop :=
+Inductive Term {lookup : Map.to Name.name} (O2O : Map.OneToOne lookup) : Term.term -> Term.term -> Prop :=
   | Err
-      : Term lookup Term.Err Term.Err
+      : Term O2O Term.Err Term.Err
   | Typ
-      : Term lookup Term.Typ Term.Typ
+      : Term O2O Term.Typ Term.Typ
   | Prp
-      : Term lookup Term.Prp Term.Prp
+      : Term O2O Term.Prp Term.Prp
   | Ctr ctor
-      : Term lookup (Term.Ctr ctor) (Term.Ctr ctor) (* constructor names live in a different universe *)
+      : Term O2O (Term.Ctr ctor) (Term.Ctr ctor) (* constructor names live in a different universe *)
   | Mov x y (F : Map.Find lookup x y)
-      : Term lookup (Term.Mov x) (Term.Mov y)
+      : Term O2O (Term.Mov x) (Term.Mov y)
   | Ref x y (F : Map.Find lookup x y)
-      : Term lookup (Term.Ref x) (Term.Ref y)
+      : Term O2O (Term.Ref x) (Term.Ref y)
   | App
-      function renamed_function (function_renaming : Term lookup function renamed_function)
-      argument renamed_argument (argument_renaming : Term lookup argument renamed_argument)
-      : Term lookup (Term.App function argument) (Term.App renamed_function renamed_argument)
+      function renamed_function (function_renaming : Term O2O function renamed_function)
+      argument renamed_argument (argument_renaming : Term O2O argument renamed_argument)
+      : Term O2O (Term.App function argument) (Term.App renamed_function renamed_argument)
   | For
-      type renamed_type (type_renaming : Term lookup type renamed_type)
-      variable unshadowed (not_shadowed : Map.OverwriteIfPresent variable variable lookup unshadowed)
-      body renamed_body (body_renaming : Term unshadowed body renamed_body)
-      : Term lookup (Term.For variable type body) (Term.For variable renamed_type renamed_body)
+      type renamed_type (type_renaming : Term O2O type renamed_type)
+      variable variable_only (only_variable : Map.Singleton variable tt variable_only)
+      unshadowed (not_shadowed : Map.OverwriteIfPresent variable variable lookup unshadowed)
+      {O2OU : Map.OneToOne unshadowed} body renamed_body (body_renaming : Term O2OU body renamed_body)
+      : Term O2O (Term.For variable type body) (Term.For variable renamed_type renamed_body)
   | Cas
-      other_cases renamed_other_cases (other_cases_renaming : Term lookup other_cases renamed_other_cases)
+      other_cases renamed_other_cases (other_cases_renaming : Term O2O other_cases renamed_other_cases)
       pattern bound_in_pattern (find_pattern_bindings : Map.Reflect (BoundIn.Pattern pattern) bound_in_pattern)
       pattern_to_self (pattern_idem : Map.ToSelf bound_in_pattern pattern_to_self)
-      unshadowed (not_shadowed : Map.BulkOverwrite pattern_to_self lookup unshadowed)
-      body_if_match renamed_body_if_match (body_if_match_renaming : Term unshadowed body_if_match renamed_body_if_match)
-      : Term lookup
+      unshadowed (not_shadowed : Map.BulkOverwrite pattern_to_self lookup unshadowed) {O2OU : Map.OneToOne unshadowed}
+      body_if_match renamed_body_if_match (body_if_match_renaming : Term O2OU body_if_match renamed_body_if_match)
+      : Term O2O
         (Term.Cas pattern body_if_match other_cases)
         (Term.Cas pattern renamed_body_if_match renamed_other_cases)
   .
-Arguments Term lookup term renamed.
+Arguments Term {lookup} O2O term renamed.
 
 
 
-Lemma term_eq {l1 t1 y1} (R1 : Term l1 t1 y1)
-  {l2} (El : Map.Eq l1 l2)
+Lemma term_eq {l1} {O2O1 : Map.OneToOne l1} {t1 y1} (R1 : Term O2O1 t1 y1)
+  {l2} (El : Map.Eq l1 l2) (O2O2 : Map.OneToOne l2)
   {t2} (Et : t1 = t2)
   {y2} (Ey : y1 = y2)
-  : Term l2 t2 y2.
+  : Term O2O2 t2 y2.
 Proof.
-  subst. rename t2 into t. rename y2 into y. generalize dependent l2. induction R1; intros.
-  - constructor.
-  - constructor.
-  - constructor.
-  - constructor.
-  - constructor. apply El. exact F.
-  - constructor. apply El. exact F.
+  subst. rename t2 into t. rename y2 into y. generalize dependent l2.
+  induction R1; intros; try solve [constructor; apply El; exact F].
   - constructor; [apply IHR1_1 | apply IHR1_2]; exact El.
-  - econstructor. { apply IHR1_1. exact El. } 2: { exact R1_2. }
-    eapply Map.overwrite_if_present_eq; try reflexivity; try eassumption. apply Map.eq_refl.
   - econstructor; try eassumption. { apply IHR1_1. exact El. }
-    eapply Map.bulk_overwrite_eq; try eassumption; apply Map.eq_refl.
+    intros k v. cbn in not_shadowed. rewrite not_shadowed. cbn in El. rewrite El. reflexivity.
+  - econstructor; try eassumption. { apply IHR1_1. exact El. }
+    intros k v. cbn in not_shadowed. rewrite not_shadowed. cbn in El. rewrite El. reflexivity.
 Qed.
 
+Lemma term_det {l1} {O2O1 : Map.OneToOne l1} {t1 y1} (R1 : Term O2O1 t1 y1)
+  {l2} (El : Map.Eq l1 l2) (O2O2 : Map.OneToOne l2)
+  {t2} (Et : t1 = t2)
+  {y2} (R2 : Term O2O2 t2 y2)
+  : y1 = y2.
+Proof.
+  subst. rename t2 into t. generalize dependent y2. generalize dependent l2.
+  induction R1; intros; try solve [invert R2; reflexivity].
+  - invert R2. f_equal. apply El in F0. eapply Map.find_det; eassumption.
+  - invert R2. f_equal. apply El in F0. eapply Map.find_det; eassumption.
+  - invert R2. f_equal; [eapply IHR1_1 | eapply IHR1_2]; eassumption.
+  - invert R2. f_equal; [eapply IHR1_1 | eapply IHR1_2]; try eassumption.
+    eapply Map.overwrite_if_present_det; try reflexivity; eassumption.
+  - invert R2. f_equal; [eapply IHR1_2 | eapply IHR1_1]; try eassumption.
+    eapply Map.bulk_overwrite_det; try reflexivity; try eassumption.
+    eapply Map.to_self_det; try eassumption.
+    intros k []; split; intro F; (eassert (I : (Map.In _ _)); [eexists; exact F |]);
+    [apply find_pattern_bindings in I | apply find_pattern_bindings0 in I];
+    [apply find_pattern_bindings0 in I | apply find_pattern_bindings in I];
+    destruct I as [[] F']; exact F'.
+Qed.
+
+Lemma term_superset {lil} {O2Ol : Map.OneToOne lil} {tl yl} (Rl : Term O2Ol tl yl)
+  {big} (S : Map.Subset lil big) (O2Ob : Map.OneToOne big)
+  (caveat : forall x (B : BoundIn.Term tl x) z (F : Map.Find big z x), z = x)
+  {tb} (Et : tl = tb)
+  {yb} (Ey : yl = yb)
+  : Term O2Ob tb yb.
+Proof.
+  subst. rename tb into t. rename yb into y. generalize dependent big. {
+  induction Rl; intros; try solve [constructor; apply S; exact F].
+  - constructor; [eapply IHRl1 | eapply IHRl2]; try exact S; intros;
+    (apply caveat; [| exact F]); [apply BoundIn.TApF | apply BoundIn.TApA]; exact B.
+  - econstructor. { apply IHRl1; intros. { exact S. } apply caveat. 2: { exact F. } apply BoundIn.TFoT. exact B. }
+    { exact only_variable. } { apply Map.overwrite_if_present_overwrite. } apply IHRl2. 2: {
+      intros. apply Map.overwrite_if_present_overwrite in F as [[-> ->] | [N F]]. { reflexivity. }
+      apply caveat. 2: { exact F. } apply BoundIn.TFoB. exact B. }
+    intros k v. cbn in not_shadowed. rewrite not_shadowed.
+    assert (A := @Map.overwrite_if_present_overwrite); cbn in A; rewrite A; clear A.
+    intros [[-> ->] | [N F]]; [left | right]; [split; reflexivity |]. split. { exact N. } apply S. exact F.
+  - econstructor. { apply IHRl1; intros. { exact S. } apply caveat. 2: { exact F. } apply BoundIn.TCaO. exact B. }
+    { eassumption. } { eassumption. } { apply Map.bulk_overwrite_bulk_overwrite. } apply IHRl2. 2: {
+      intros. apply Map.bulk_overwrite_bulk_overwrite in F as [F | [N F]].
+      + apply pattern_idem in F as [I ->]. reflexivity.
+      + apply caveat. 2: { exact F. } apply BoundIn.TCaB. exact B. }
+    intros k v. cbn in not_shadowed. rewrite not_shadowed.
+    assert (A := @Map.bulk_overwrite_bulk_overwrite); cbn in A; rewrite A; clear A.
+    intros [F | [N F]]; [left; exact F | right]. split. { exact N. } apply S. exact F. }
+  Unshelve.
+  - eapply Map.one_to_one_overwrite. { apply Map.overwrite_if_present_overwrite. }
+    split; intros. { eapply O2Ob; eassumption. } apply caveat. { constructor. } exact F.
+  - eapply Map.one_to_one_bulk_overwrite. { apply Map.bulk_overwrite_bulk_overwrite. }
+    split. { cbn. intros. apply pattern_idem in F1 as [I1 ->]. apply pattern_idem in F2 as [I2 ->]. reflexivity. }
+    split; intros. { eapply O2Ob; eassumption. } apply pattern_idem in Ff as [If ->].
+    apply caveat. 2: { exact Fo. } apply BoundIn.TCaP. apply find_pattern_bindings. exact If.
+Qed.
+
+Lemma term_then_in_domain {lookup} {O2O : Map.OneToOne lookup} {term renamed_term} (T : Term O2O term renamed_term)
+  {x} (U : UsedIn.Term term x)
+  : Map.In lookup x.
+Proof.
+  generalize dependent x. induction T; intros; invert U.
+  - eexists. exact F.
+  - eexists. exact F.
+  - apply IHT1. exact used_in_function.
+  - apply IHT2. exact used_in_argument.
+  - apply IHT1. exact used_in_type.
+  - apply IHT2 in used_in_body as [y F]. apply not_shadowed in F as [[-> ->] | [N F]].
+    + contradiction not_shadowed0. reflexivity.
+    + eexists. exact F.
+  - apply IHT2 in used_in_body as [y F]. apply not_shadowed in F as [F | [N F]].
+    + contradiction not_shadowed0. apply find_pattern_bindings. apply pattern_idem in F as [I ->]. exact I.
+    + eexists. exact F.
+  - apply IHT1. exact used_in_another_case.
+Qed.
+
+Lemma term_then_in_range {lookup} {O2O : Map.OneToOne lookup} {term renamed_term} (T : Term O2O term renamed_term)
+  {x} (U : UsedIn.Term renamed_term x)
+  : Map.InRange lookup x.
+Proof.
+  generalize dependent x. induction T; intros; invert U.
+  - eexists. exact F.
+  - eexists. exact F.
+  - apply IHT1. exact used_in_function.
+  - apply IHT2. exact used_in_argument.
+  - apply IHT1. exact used_in_type.
+  - apply IHT2 in used_in_body as [y F]. apply not_shadowed in F as [[-> ->] | [N F]].
+    + contradiction not_shadowed0. reflexivity.
+    + eexists. exact F.
+  - apply IHT2 in used_in_body as [y F]. apply not_shadowed in F as [F | [N F]].
+    + contradiction not_shadowed0. apply find_pattern_bindings. apply pattern_idem in F as [I ->]. exact I.
+    + eexists. exact F.
+  - apply IHT1. exact used_in_another_case.
+Qed.
+
+(*
+Lemma term_reversible_bwd {lookup} (O2O : Map.OneToOne lookup) {term renamed_term} (fwd : Term O2O term renamed_term)
+  : exists undo (O2OU : Map.OneToOne undo), (
+      Term O2OU renamed_term term /\
+      (forall x, Map.In undo x <-> UsedIn.Term renamed_term x)
+    ).
+Proof.
+  induction fwd; try solve [exists Map.empty; exists Map.one_to_one_empty; split; intros; [constructor |];
+    split; [intro I; apply Map.empty_empty in I as [] | intro U; invert U]].
+  - eexists. eexists (Map.one_to_one_singleton _ _). split; intros. { constructor. apply Map.find_singleton. split; reflexivity. }
+    split. { intro I. apply Map.in_singleton in I as ->. constructor. } intro U. invert U. apply Map.in_singleton. reflexivity.
+  - eexists. eexists (Map.one_to_one_singleton _ _). split; intros. { constructor. apply Map.find_singleton. split; reflexivity. }
+    split. { intro I. apply Map.in_singleton in I as ->. constructor. } intro U. invert U. apply Map.in_singleton. reflexivity.
+  - destruct IHfwd1 as [mf [Of [Rf Df]]]. destruct IHfwd2 as [ma [Oa [Ra Da]]].
+    exists (Map.overriding_union mf ma). eexists. split.
+    + constructor; (eapply term_superset; try reflexivity; try eassumption).
+      * cbn. intros. eapply Map.union_overriding. 2: { left. exact F. } cbn. intros.
+        assert (Uf : UsedIn.Term renamed_function k0). { apply Df. eexists. exact F0. }
+        assert (Ua : UsedIn.Term renamed_argument k0). { apply Da. eexists. exact F1. }
+        (* I think this could have been bound way above so it's not an absurd case--we just need to ensure cross-branch consistency *)
 
 
+
+  split; intro T.
+  - generalize dependent inverted. induction T; intros; try solve [constructor; apply inv; exact F].
+    + constructor; [apply IHT1 | apply IHT2]; exact inv.
+    + econstructor. { apply IHT1. exact inv. } { eassumption. } { apply Map.overwrite_if_present_overwrite. }
+      Unshelve. 2: { eapply Map.one_to_one_overwrite. { apply Map.overwrite_if_present_overwrite. } split; intros.
+      * apply inv in F1. apply inv in F2. eapply Map.find_det; eassumption.
+      * apply inv in F.
+      eapply IHT2.
+
+
+
+      asdf.
+      apply IHT2. intros k v. cbn in not_shadowed; rewrite not_shadowed.
+      assert (A := @Map.overwrite_if_present_overwrite); cbn in A; rewrite A; clear A. cbn in inv; rewrite <- inv.
+      split; (intros [[-> ->] | [N F]]; [left; split; reflexivity | right]); (split; [| exact F]); intros ->.
+      * apply N. eapply O2OU; apply not_shadowed. 2: { left. split; reflexivity. } right. split; assumption.
+      * assert (copy := O2OU). eapply Map.one_to_one_overwrite in copy as [D E]. 2: { exact not_shadowed. }
+        apply N in E as [].
+
+        assert (A : Map.Find unshadowed variable v). { apply not_shadowed. left.
+Qed.
+
+Lemma term_reversible {lookup} (O2O : Map.OneToOne lookup) term renamed_term
+  : Term O2O term renamed_term <-> exists undo (O2OU : Map.OneToOne undo), Term O2OU renamed_term term.
+*)
+
+
+
+(*
 (* TODO: Grammar: should this have an `e`? I'm leaning toward yes. *)
 Definition RenameableTerm (lookup : Map.to Name.name) term : Prop :=
+  Map.OneToOne lookup /\
+  (forall v (B : BoundIn.Term term v) k (F : Map.Find lookup k v), k = v) /\ (* can't rename an unbound variable into a bound one *)
   forall x (U : UsedIn.Term term x), Map.In lookup x.
 Arguments RenameableTerm lookup term/.
 
 Lemma renameable_term lookup term
-  : (exists renamed, Term lookup term renamed) <-> RenameableTerm lookup term.
+  : (exists (O2O : Map.OneToOne lookup) renamed, Term O2O term renamed) <-> RenameableTerm lookup term.
 Proof.
   cbn. split.
-  - intros [renamed R]; intros. induction R.
-    + invert U.
-    + invert U.
-    + invert U.
-    + invert U.
-    + invert U. eexists. exact F.
-    + invert U. eexists. exact F.
-    + invert U; [apply IHR1 | apply IHR2]; assumption.
-    + invert U. { apply IHR1. assumption. } specialize (IHR2 used_in_body) as [y IH].
-      apply not_shadowed in IH as [[-> ->] | [N F]]. { contradiction not_shadowed0. reflexivity. } eexists. exact F.
-    + invert U. 2: { apply IHR1. exact used_in_another_case. } specialize (IHR2 used_in_body) as [y IH].
-      apply not_shadowed in IH as [F | [N F]]. 2: { eexists. exact F. }
-      apply pattern_idem in F as [I ->]. apply find_pattern_bindings in I. apply not_shadowed0 in I as [].
-  - intros I. generalize dependent lookup. induction term; intros.
-    + eexists. constructor.
-    + eexists. constructor.
-    + eexists. constructor.
-    + eexists. constructor.
-    + edestruct I as [y F]. { constructor. } eexists. constructor. exact F.
-    + edestruct I as [y F]. { constructor. } eexists. constructor. exact F.
-    + edestruct IHterm1 as [rf IHf]. { intros. apply I. apply UsedIn.ApF. exact U. }
-      edestruct IHterm2 as [ra IHa]. { intros. apply I. apply UsedIn.ApA. exact U. }
-      eexists. constructor; [exact IHf | exact IHa].
-    + edestruct IHterm1 as [rt IHt]. { intros. apply I. apply UsedIn.FoT. exact U. }
-      edestruct IHterm2 as [rb IHb]. 2: {
-        eexists. econstructor; try eassumption. apply Map.overwrite_if_present_overwrite. }
-      intros. eapply Map.in_overwrite_if_present. { apply Map.overwrite_if_present_overwrite. }
-      destruct (Name.spec x variable); [left | right]. { exact Y. } apply I. apply UsedIn.FoB; assumption.
-    + edestruct IHterm2 as [ro IHo]. { intros. apply I. apply UsedIn.CaO. exact U. }
-      edestruct IHterm1 as [rb IHb]. 2: {
-        eexists. econstructor; try eassumption. { apply BoundIn.pattern_spec. } { apply Map.to_self_to_self. }
-        apply Map.bulk_overwrite_bulk_overwrite. }
-      intros. eapply Map.in_bulk_overwrite. { apply Map.bulk_overwrite_bulk_overwrite. }
+  - intros [O2O [renamed R]]; intros. split. { exact O2O. }
+    induction R; intros; try solve [split; intros; [invert B | invert U]].
+    + split; intros.
+      * invert B.
+      * invert U. eexists. exact F.
+    + split; intros.
+      * invert B.
+      * invert U. eexists. exact F.
+    + split; intros.
+      * invert B; [eapply IHR1 | eapply IHR2]; eassumption.
+      * invert U; [apply IHR1 | apply IHR2]; assumption.
+    + split; intros.
+      * invert B.
+        -- eapply O2OU; apply not_shadowed. 2: { left. split; reflexivity. }
+           destruct (Name.spec k v); [left | right]. { subst. split; reflexivity. }
+           split. { exact N. } exact F.
+        -- apply IHR1. { exact bound_in_type. } exact F.
+        -- destruct (Name.spec k variable). 2: { apply IHR2. { exact bound_in_body. }
+             apply not_shadowed. right. split. { exact N. } exact F. }
+           subst.
+           (* Definition is not precise enough: we can't map *to* a term that's bound
+            * ... *UNLESS* what it's bound *from* is bound *first*,
+            * in which case it's kicked out of the mappings before it's a problem.
+            * But writing that down is just as hard as trying the actual thing. *)
+Qed.
+*)
+
+
+
+(* The above complication--that the exact conditions determining whether a term is renameable is just as complex as renaming them--
+ * means that we can't have bidirectional implication, but being slightly too cautious makes the permissive case easy to prove: *)
+Definition ExtraSafe (lookup : Map.to Name.name) term : Prop :=
+  Map.OneToOne lookup /\
+  (forall v (B : BoundIn.Term term v) k (F : Map.Find lookup k v), k = v) /\ (* can't rename an unbound variable into a bound one *)
+  forall x (U : UsedIn.Term term x), Map.In lookup x.
+
+(* TODO: Grammar: should this have an `e`? I'm leaning toward yes. *)
+Lemma renameable lookup term (safe : ExtraSafe lookup term)
+  : exists (O2O : Map.OneToOne lookup) renamed_term, Term O2O term renamed_term.
+Proof.
+  destruct safe as [O2O [no_capture covering]]. exists O2O. { generalize dependent lookup.
+  induction term; intros; try solve [eexists; constructor].
+  - edestruct covering as [y F]. { constructor. } eexists. constructor. exact F.
+  - edestruct covering as [y F]. { constructor. } eexists. constructor. exact F.
+  - edestruct IHterm1; [| | edestruct IHterm2; [| | eexists; constructor; eassumption]]; intros.
+    + apply no_capture. { apply BoundIn.TApF. exact B. } exact F.
+    + apply covering. apply UsedIn.ApF. exact U.
+    + apply no_capture. { apply BoundIn.TApA. exact B. } exact F.
+    + apply covering. apply UsedIn.ApA. exact U.
+  - edestruct IHterm1; [| | edestruct IHterm2; [| | eexists; econstructor; try eassumption]]; intros.
+    5: { apply Map.singleton_singleton. } 5: { apply Map.overwrite_if_present_overwrite. }
+    + apply no_capture. { apply BoundIn.TFoT. exact B. } exact F.
+    + apply covering. apply UsedIn.FoT. exact U.
+    + apply Map.overwrite_if_present_overwrite in F as [[-> ->] | [N F]]. { reflexivity. }
+      apply no_capture. { apply BoundIn.TFoB. exact B. } exact F.
+    + eapply Map.in_overwrite_if_present. { apply Map.overwrite_if_present_overwrite. }
+      destruct (Name.spec x0 variable); [left | right]. { exact Y. }
+      apply covering. apply UsedIn.FoB. { exact N. } exact U.
+  - edestruct IHterm1; [| | edestruct IHterm2; [| | eexists; econstructor; try eassumption]]; intros.
+    5: { apply BoundIn.pattern_spec. } 5: { apply Map.to_self_to_self. } 5: { apply Map.bulk_overwrite_bulk_overwrite. }
+    + apply Map.bulk_overwrite_bulk_overwrite in F as [F | [N F]].
+      * apply Map.to_self_to_self in F as [F ->]. reflexivity.
+      * apply no_capture. { apply BoundIn.TCaB. exact B. } exact F.
+    + eapply Map.in_bulk_overwrite. { apply Map.bulk_overwrite_bulk_overwrite. }
       rewrite Map.in_to_self. destruct (Map.in_spec (BoundIn.pattern pattern0) x); [left | right]. { exact Y. }
-      split. { exact N. } apply I. apply UsedIn.CaB. 2: { exact U. }
+      split. { exact N. } apply covering. apply UsedIn.CaB. 2: { exact U. }
       intro B. apply N. apply BoundIn.pattern_spec. exact B.
+    + apply no_capture. { apply BoundIn.TCaO. exact B. } exact F.
+    + apply covering. apply UsedIn.CaO. exact U. }
+  Unshelve.
+  - eapply Map.one_to_one_overwrite. { apply Map.overwrite_if_present_overwrite. }
+    split; intros. { eapply O2O; eassumption. } apply no_capture. { constructor. } exact F.
+  - eapply Map.one_to_one_bulk_overwrite. { apply Map.bulk_overwrite_bulk_overwrite. }
+    split; [| split]; intros. { apply Map.one_to_one_to_self. } { eapply O2O; eassumption. }
+    apply Map.to_self_to_self in Ff as [If ->]. eapply no_capture. 2: { exact Fo. }
+    apply BoundIn.TCaP. apply BoundIn.pattern_spec. exact If.
 Qed.
 
 
@@ -366,70 +594,105 @@ Fixpoint term lookup t :=
   | _ => Some t
   end.
 
-Lemma term_spec lookup t
-  : Reflect.Option (Term lookup t) (term lookup t).
+Lemma term_spec {lookup t} (safe : ExtraSafe lookup t)
+  : Reflect.Option (fun renamed_term => exists O2O : Map.OneToOne lookup, Term O2O t renamed_term) (term lookup t).
 Proof.
-  generalize dependent lookup. induction t; intros; cbn in *; try solve [repeat constructor].
-  - destruct (Map.find_spec lookup name); constructor. { constructor. exact Y. }
-    intros t C. invert C. apply N in F as [].
-  - destruct (Map.find_spec lookup name); constructor. { constructor. exact Y. }
-    intros t C. invert C. apply N in F as [].
-  - destruct (IHt1 lookup). 2: { constructor. intros t C. invert C. apply N in function_renaming as []. }
-    destruct (IHt2 lookup); constructor. { constructor; assumption. }
-    intros t C. invert C. apply N in argument_renaming as [].
-  - destruct (IHt1 lookup). 2: { constructor. intros t C. invert C. apply N in type_renaming as []. }
-    destruct (IHt2 (Map.overriding_add variable variable lookup)); constructor. {
-      econstructor; try eassumption. apply Map.overwrite_if_present_overwrite. }
-    intros t C. invert C. eapply N. eapply term_eq; try reflexivity; try eassumption.
-    eapply Map.overwrite_if_present_det; try reflexivity; try eassumption. { apply Map.eq_refl. }
-    apply Map.overwrite_if_present_overwrite.
-  - destruct (IHt2 lookup). 2: { constructor. intros t C. invert C. apply N in other_cases_renaming as []. }
-    fold (Map.to_self (BoundIn.pattern pattern0)).
-    destruct (IHt1 (Map.overriding_union (Map.to_self (BoundIn.pattern pattern0)) lookup)); constructor. {
-      econstructor; try eassumption. { apply BoundIn.pattern_spec. } { apply Map.to_self_to_self. }
-      apply Map.bulk_overwrite_bulk_overwrite. }
-    intros t R. invert R. eapply N. eapply term_eq; try reflexivity. { exact body_if_match_renaming. }
-    eapply Map.bulk_overwrite_det. { exact not_shadowed. } 3: { apply Map.bulk_overwrite_bulk_overwrite. }
-    2: { apply Map.eq_refl. } eapply Map.to_self_det; try eassumption. 2: { apply Map.to_self_to_self. }
-    intros x' y'. split; intro F; (eassert (I : Map.In _ _); [eexists; exact F |]).
-    + eapply find_pattern_bindings in I. apply BoundIn.pattern_spec in I. destruct I as [[] I]. destruct y'. exact I.
-    + apply BoundIn.pattern_spec in I. apply find_pattern_bindings in I. destruct I as [[] I]. destruct y'. exact I.
+  destruct safe as [O2O [no_capture covering]]. generalize dependent lookup. {
+  induction t; intros; simpl term; try solve [constructor; exists O2O; constructor].
+  - destruct (Map.find_spec lookup name); constructor. { exists O2O. constructor. exact Y. }
+    intros t [O2O' C]. invert C. apply N in F as [].
+  - destruct (Map.find_spec lookup name); constructor. { exists O2O. constructor. exact Y. }
+    intros t [O2O' C]. invert C. apply N in F as [].
+  - destruct (IHt1 _ O2O); intros.
+    + apply no_capture. { apply BoundIn.TApF. exact B. } exact F.
+    + apply covering. apply UsedIn.ApF. exact U.
+    + destruct (IHt2 _ O2O); intros.
+      * apply no_capture. { apply BoundIn.TApA. exact B. } exact F.
+      * apply covering. apply UsedIn.ApA. exact U.
+      * constructor. exists O2O. destruct Y. destruct Y0.
+        constructor; eapply term_eq; try reflexivity; try eassumption; apply Map.eq_refl.
+      * constructor. intros renamed [O2O' C]. invert C. eapply N. eexists. eassumption.
+    + constructor. intros renamed [O2O' C]. invert C. eapply N. eexists. eassumption.
+  - destruct (IHt1 _ O2O); intros.
+    + apply no_capture. { apply BoundIn.TFoT. exact B. } exact F.
+    + apply covering. apply UsedIn.FoT. exact U.
+    + edestruct (IHt2 (Map.overriding_add variable variable lookup)); intros.
+      * eapply Map.one_to_one_overwrite. { apply Map.overwrite_if_present_overwrite. }
+        split; intros. { eapply O2O; eassumption. } apply no_capture. { constructor. } exact F.
+      * apply Map.find_overriding_add in F as [[-> ->] | [N F]]. { reflexivity. }
+        apply no_capture. { apply BoundIn.TFoB. exact B. } exact F.
+      * apply Map.in_overriding_add. destruct (Name.spec x0 variable); [left | right]. { assumption. }
+        apply covering. apply UsedIn.FoB. { exact N. } exact U.
+      * constructor. exists O2O. destruct Y. destruct Y0. econstructor.
+        -- eapply term_eq; try reflexivity. { eassumption. } apply Map.eq_refl.
+        -- apply Map.singleton_singleton.
+        -- apply Map.overwrite_if_present_overwrite.
+        -- eassumption.
+      * constructor. intros renamed [O2O' C]. invert C. eapply N.
+        eexists. eapply term_eq; try reflexivity. { exact body_renaming. }
+        intros k v. cbn in not_shadowed. rewrite not_shadowed. rewrite Map.find_overriding_add. reflexivity.
+    + constructor. intros renamed [O2O' C]. invert C. eapply N. eexists. eassumption.
+  - destruct (IHt2 _ O2O); intros.
+    + apply no_capture. { apply BoundIn.TCaO. exact B. } exact F.
+    + apply covering. apply UsedIn.CaO. exact U.
+    + edestruct (IHt1 (Map.overriding_union (Map.map (fun k _ => k) (BoundIn.pattern pattern0)) lookup)); intros.
+      * eapply Map.one_to_one_bulk_overwrite. { apply Map.bulk_overwrite_bulk_overwrite. }
+        split. { apply Map.one_to_one_to_self. } split; intros. { eapply O2O; eassumption. }
+        apply Map.to_self_to_self in Ff as [If ->]. apply no_capture. 2: { exact Fo. }
+        apply BoundIn.TCaP. apply BoundIn.pattern_spec. exact If.
+      * apply Map.bulk_overwrite_bulk_overwrite in F as [F | [N F]].
+        -- apply Map.to_self_to_self in F as [I ->]. reflexivity.
+        -- apply no_capture. { apply BoundIn.TCaB. exact B. } exact F.
+      * fold (Map.to_self (BoundIn.pattern pattern0)).
+        eapply Map.in_bulk_overwrite. { apply Map.bulk_overwrite_bulk_overwrite. }
+        rewrite Map.in_to_self. destruct (Map.in_spec (BoundIn.pattern pattern0) x0); [left | right]. { assumption. }
+        split. { exact N. } apply covering. apply UsedIn.CaB. 2: { exact U. }
+        intro B. apply N. apply BoundIn.pattern_spec. exact B.
+      * constructor. exists O2O. destruct Y. destruct Y0. econstructor.
+        -- eapply term_eq; try reflexivity. { eassumption. } apply Map.eq_refl.
+        -- apply BoundIn.pattern_spec.
+        -- apply Map.to_self_to_self.
+        -- apply Map.bulk_overwrite_bulk_overwrite.
+        -- eassumption.
+      * constructor. intros renamed [O2O' C]. invert C. eapply N.
+        eexists. eapply term_eq; try reflexivity. { exact body_if_match_renaming. }
+        fold (Map.to_self (BoundIn.pattern pattern0)). intros k v. cbn in not_shadowed. rewrite not_shadowed.
+        assert (A := @Map.bulk_overwrite_bulk_overwrite); cbn in A; rewrite A; clear A.
+        split; (intros [F | [N' F]]; [left | right]).
+        -- apply Map.to_self_to_self. apply pattern_idem in F as [I ->]. apply find_pattern_bindings in I.
+           apply BoundIn.pattern_spec in I. split. { assumption. } reflexivity.
+        -- split. 2: { exact F. } intros [v' F']. apply Map.to_self_to_self in F' as [I' ->].
+           apply BoundIn.pattern_spec in I'. apply find_pattern_bindings in I'.
+           apply N'. exists v'. apply pattern_idem. split. { exact I'. } reflexivity.
+        -- apply pattern_idem. apply Map.to_self_to_self in F as [I ->]. apply BoundIn.pattern_spec in I.
+           apply find_pattern_bindings in I. split. { exact I. } reflexivity.
+        -- split. 2: { exact F. } intros [v' F']. apply pattern_idem in F' as [I' ->].
+           apply find_pattern_bindings in I'. apply BoundIn.pattern_spec in I'. eapply N'.
+           exists v'. apply Map.to_self_to_self. split. { exact I'. } reflexivity.
+    + constructor. intros renamed [O2O' C]. invert C. eapply N. eexists. eassumption. }
+  Unshelve.
+  - eapply Map.one_to_one_overwrite. { apply Map.overwrite_if_present_overwrite. }
+    split; intros. { eapply O2O; eassumption. } apply no_capture. { constructor. } exact F.
+  - eapply Map.one_to_one_bulk_overwrite. { apply Map.bulk_overwrite_bulk_overwrite. }
+    split. { apply Map.one_to_one_to_self. } split; intros. { eapply O2O; eassumption. }
+    apply Map.to_self_to_self in Ff as [If ->]. apply no_capture. 2: { exact Fo. }
+    apply BoundIn.TCaP. apply BoundIn.pattern_spec. exact If.
 Qed.
 
-Lemma term_det
-  {l1 t1 r1} (T1 : Term l1 t1 r1)
-  {l2} (El : Map.Eq l1 l2)
-  {t2} (Et : t1 = t2)
-  {r2} (T2 : Term l2 t2 r2)
-  : r1 = r2.
+Lemma term_iff {lookup t} (safe : ExtraSafe lookup t) renamed_t
+  : term lookup t = Some renamed_t <-> exists O2O : Map.OneToOne lookup, Term O2O t renamed_t.
 Proof.
-  subst. generalize dependent r2. generalize dependent l2. induction T1; intros; invert T2; try reflexivity.
-  - f_equal. eapply Map.find_det. { eassumption. } apply El. assumption.
-  - f_equal. eapply Map.find_det. { eassumption. } apply El. assumption.
-  - f_equal; [eapply IHT1_1 | eapply IHT1_2]; eassumption.
-  - f_equal. { eapply IHT1_1; eassumption. } eapply IHT1_2. 2: { eassumption. }
-    eapply Map.overwrite_if_present_det; try reflexivity; eassumption.
-  - f_equal. 2: { eapply IHT1_1; eassumption. } eapply IHT1_2. 2: { eassumption. }
-    eapply Map.bulk_overwrite_det; try reflexivity; try eassumption.
-    eapply Map.to_self_det; try eassumption. intros x [].
-    split; intro F; (eassert (I : Map.In _ _); [eexists; exact F |]);
-    [apply find_pattern_bindings in I | apply find_pattern_bindings0 in I];
-    [apply find_pattern_bindings0 in I | apply find_pattern_bindings in I];
-    destruct I as [[] F']; exact F'.
-Qed.
-
-Lemma term_iff lookup t renamed_t
-  : Term lookup t renamed_t <-> term lookup t = Some renamed_t.
-Proof.
-  destruct (term_spec lookup t).
-  - split. 2: { intro E. invert E. exact Y. }
-    intro T. f_equal. eapply term_det; try reflexivity; try eassumption. apply Map.eq_refl.
-  - split. { intro T. apply N in T as []. } intro D. discriminate D.
+  destruct (term_spec safe). 2: { split. { intro D. discriminate D. } intro C. apply N in C as []. }
+  split. { intro E. invert E. exact Y. } intros [O2O T]. destruct Y as [O2O' T']. f_equal.
+  eapply term_det; try reflexivity; try eassumption. apply Map.eq_refl.
 Qed.
 
 
 
-Definition Context (lookup : Map.to Name.name) (context : Context.context) (renamed_context : Context.context) : Prop :=
-  forall k' v', Map.Find renamed_context k' v' <-> exists k, (Map.Find lookup k k' /\
-    exists v, (Term lookup v v' /\ Map.Find context k v)).
-Arguments Context lookup context renamed_context/.
+Definition Context {lookup : Map.to Name.name} (O2O : Map.OneToOne lookup)
+  (context : Context.context) (renamed_context : Context.context) : Prop :=
+  (*forall k' v', Map.Find renamed_context k' v' <-> exists k, (Map.Find lookup k k' /\*)
+  (*  exists v, (Term lookup v v' /\ Map.Find context k v)).*)
+  forall name term, Map.Find context name term <-> exists renamed_name, (Map.Find lookup name renamed_name /\
+    exists renamed_term, (Term O2O term renamed_term /\ Map.Find renamed_context renamed_name renamed_term)).
+Arguments Context {lookup} O2O context renamed_context/.
